\pdfoutput=1
\documentclass[a4paper,pdftex,10pt]{article}
\input{preable_pdflatex.tex}
\begin{document}

\maketitle

\tableofcontents

% ----------------------------------------------------------------------------------------------------
\clearpage
\section{Problem 1*}

The Christoffel symbol is defined as
\begin{equation}
  \Gamma_{\mu\alpha\beta}
  =
  \frac{1}{2}
  \left(
  \pdv{g_{\mu\alpha}}{x^{\beta}}
  +
  \pdv{g_{\mu\beta}}{x^{\alpha}}
  -
  \pdv{g_{\alpha\beta}}{x^{\mu}}
  \right)
  \label{eqn:christoffel_symbol}
\end{equation}
in a coordinate system $x^{\lambda}$ and transform into a system $\tilde{x}^{\lambda}$\footnote{
  In the problem statement, we should consider the transformation $x^{\lambda}$ into a system "${x^{\prime}}^{\lambda}$" but I should apologize since we will use a different label "$\tilde{x}^{\lambda}$", though it is trivial.
}. The transformation laws of the coordinate are
\begin{align}
  g^{\mu\nu}
   & =
  \pdv{x^{\mu}}{\tilde{x}^{\rho}}\pdv{x^{\nu}}{\tilde{x}^{\sigma}}\tilde{g}^{\rho\sigma}
  \\
  \pdv{}{x^{\mu}}
   & =
  \pdv{\tilde{x}^{\lambda}}{x^{\mu}}\pdv{}{\tilde{x}^{\lambda}}  .
\end{align}
Putting these relations into the definition \eqref{eqn:christoffel_symbol}, we obtain the transformation law
\begin{align}
  \Gamma_{\mu\alpha\beta}
   & =
  \frac{1}{2}
  \left(
  \pdv{g_{\mu\alpha}}{x^{\beta}}
  +
  \pdv{g_{\mu\beta}}{x^{\alpha}}
  -
  \pdv{g_{\alpha\beta}}{x^{\mu}}
  \right)
  \nonumber
  \\
   & =
  \frac{1}{2}
  \left\{
  \pdv{\tilde{x}^{\delta}}{x^{\beta}}\pdv{}{\tilde{x}^{\delta}}
  \left(
  \pdv{\tilde{x}^{\lambda}}{x^{\mu}}\pdv{\tilde{x}^{\gamma}}{x^{\alpha}}g_{\lambda\gamma}
  \right)
  +
  \pdv{\tilde{x}^{\gamma}}{x^{\alpha}}\pdv{}{\tilde{x}^{\gamma}}
  \left(
  \pdv{\tilde{x}^{\lambda}}{x^{\mu}}\pdv{\tilde{x}^{\delta}}{x^{\beta}}g_{\lambda\delta}
  \right)
  -
  \pdv{\tilde{x}^{\lambda}}{x^{\mu}}\pdv{}{\tilde{x}^{\lambda}}
  \left(
  \pdv{\tilde{x}^{\gamma}}{x^{\alpha}}\pdv{\tilde{x}^{\delta}}{x^{\beta}}g_{\gamma\delta}
  \right)
  \nonumber
  \right\}
  \nonumber
  \\
   & =
  \frac{1}{2}
  \left\{
  \pdv{\tilde{x}^{\delta}}{x^{\beta}}\pdv{}{\tilde{x}^{\delta}}
  \left( \pdv{\tilde{x}^{\lambda}}{x^{\mu}} \right)
  \pdv{\tilde{x}^{\gamma}}{x^{\alpha}}g_{\lambda\gamma}
  +
  \pdv{\tilde{x}^{\delta}}{x^{\beta}}
  \pdv{\tilde{x}^{\lambda}}{x^{\mu}}
  \pdv{}{\tilde{x}^{\delta}}
  \left(  \pdv{\tilde{x}^{\gamma}}{x^{\alpha}} \right)
  g_{\lambda\gamma}
  +
  \uwave{
    \pdv{\tilde{x}^{\delta}}{x^{\beta}}
    \pdv{\tilde{x}^{\lambda}}{x^{\mu}}\pdv{\tilde{x}^{\gamma}}{x^{\alpha}}
    \pdv{g_{\lambda\gamma}}{\tilde{x}^{\delta}}
  }
  \right.
  \nonumber
  \\
   & \qquad
  +
  \pdv{\tilde{x}^{\gamma}}{x^{\alpha}}\pdv{}{\tilde{x}^{\gamma}}
  \left(
  \pdv{\tilde{x}^{\lambda}}{x^{\mu}}
  \right)
  \pdv{\tilde{x}^{\delta}}{x^{\beta}}g_{\lambda\delta}
  +
  \pdv{\tilde{x}^{\gamma}}{x^{\alpha}}\pdv{}{\tilde{x}^{\gamma}}
  \pdv{\tilde{x}^{\lambda}}{x^{\mu}}
  \left(  \pdv{\tilde{x}^{\delta}}{x^{\beta}}
  \right)
  g_{\lambda\delta}
  +
  \uwave{
    \pdv{\tilde{x}^{\gamma}}{x^{\alpha}}
    \pdv{\tilde{x}^{\lambda}}{x^{\mu}}\pdv{\tilde{x}^{\delta}}{x^{\beta}}
    \pdv{g_{\lambda\delta}}{\tilde{x}^{\gamma}}
  }
  \nonumber
  \\
   & \qquad
  \left.
  -
  \pdv{\tilde{x}^{\lambda}}{x^{\mu}}\pdv{}{\tilde{x}^{\lambda}}
  \left(
  \pdv{\tilde{x}^{\gamma}}{x^{\alpha}}
  \right)
  \pdv{\tilde{x}^{\delta}}{x^{\beta}}g_{\gamma\delta}
  -
  \pdv{\tilde{x}^{\lambda}}{x^{\mu}}\pdv{\tilde{x}^{\gamma}}{x^{\alpha}}
  \pdv{}{\tilde{x}^{\lambda}}
  \left(
  \pdv{\tilde{x}^{\delta}}{x^{\beta}}
  \right)
  g_{\gamma\delta}
  -
  \uwave{
    \pdv{\tilde{x}^{\lambda}}{x^{\mu}}
    \pdv{\tilde{x}^{\gamma}}{x^{\alpha}}\pdv{\tilde{x}^{\delta}}{x^{\beta}}
    \pdv{g_{\gamma\delta}}{\tilde{x}^{\lambda}}
  }
  \right\}
  .
  \label{eqn:1}
\end{align}
The waved terms $\uwave{\qquad}$ in \eqref{eqn:1} become a twice of the Christoffel symbol:
\begin{equation}
  \pdv{\tilde{x}^{\delta}}{x^{\beta}}
  \pdv{\tilde{x}^{\lambda}}{x^{\mu}}\pdv{\tilde{x}^{\gamma}}{x^{\alpha}}
  \pdv{g_{\lambda\gamma}}{\tilde{x}^{\delta}}
  +
  \pdv{\tilde{x}^{\gamma}}{x^{\alpha}}
  \pdv{\tilde{x}^{\lambda}}{x^{\mu}}\pdv{\tilde{x}^{\delta}}{x^{\beta}}
  \pdv{g_{\lambda\delta}}{\tilde{x}^{\gamma}}
  -
  \pdv{\tilde{x}^{\lambda}}{x^{\mu}}
  \pdv{\tilde{x}^{\gamma}}{x^{\alpha}}\pdv{\tilde{x}^{\delta}}{x^{\beta}}
  \pdv{g_{\gamma\delta}}{\tilde{x}^{\lambda}}
  =
  2
  \pdv{\tilde{x}^{\lambda}}{x^{\mu}}
  \pdv{\tilde{x}^{\gamma}}{x^{\alpha}}\pdv{\tilde{x}^{\delta}}{x^{\beta}}
  \tilde{\Gamma}_{\lambda\gamma\delta}
  .
\end{equation}
But we know that there are additional terms in \eqref{eqn:1} and they violate the transformation law of the 3-rank covariant tensor. Thus we find the law as
\begin{align}
  \Gamma_{\mu\alpha\beta}
   & =
  \pdv{\tilde{x}^{\lambda}}{x^{\mu}}
  \pdv{\tilde{x}^{\gamma}}{x^{\alpha}}\pdv{\tilde{x}^{\delta}}{x^{\beta}}
  \tilde{\Gamma}_{\lambda\gamma\delta}
  +
  \frac{1}{2}
  \left\{
  \pdv{\tilde{x}^{\delta}}{x^{\beta}}\pdv{x^{\epsilon}}{\tilde{x}^{\delta}}
  \left(
  \pdv{\tilde{x}^{\lambda}}{x^{\epsilon}}{x^{\mu}}\pdv{\tilde{x}^{\gamma}}{x^{\alpha}}
  +
  \pdv{\tilde{x}^{\lambda}}{x^{\mu}}\pdv{\tilde{x}^{\gamma}}{x^{\epsilon}}{x^{\alpha}}
  \right)g_{\lambda\gamma}
  \right.
  \nonumber
  \\
   & \qquad
  +
  \pdv{\tilde{x}^{\gamma}}{x^{\alpha}}\pdv{x^{\epsilon}}{\tilde{x}^{\gamma}}
  \left(
  \pdv{\tilde{x}^{\lambda}}{x^{\mu}}{x^{\epsilon}}
  \pdv{\tilde{x}^{\delta}}{x^{\beta}}
  +
  \pdv{\tilde{x}^{\delta}}{x^{\mu}}{x^{\epsilon}}\pdv{\tilde{x}^{\lambda}}{x^{\beta}}
  \right)
  g_{\lambda\delta}
  \nonumber
  \\
   & \qquad
  \left.
  -
  \pdv{\tilde{x}^{\lambda}}{x^{\mu}}\pdv{x^{\epsilon}}{\tilde{x}^{\lambda}}
  \left(
  \pdv{\tilde{x}^{\gamma}}{x^{\epsilon}}{x^{\alpha}}\pdv{\tilde{x}^{\delta}}{x^{\beta}}
  +
  \pdv{\tilde{x}^{\gamma}}{x^{\beta}}\pdv{\tilde{x}^{\delta}}{x^{\epsilon}}{x^{\alpha}}
  \right)
  g_{\gamma\delta}
  \right\}
  \nonumber
  \\
   & =
  \pdv{\tilde{x}^{\lambda}}{x^{\mu}}
  \pdv{\tilde{x}^{\gamma}}{x^{\alpha}}\pdv{\tilde{x}^{\delta}}{x^{\beta}}
  \tilde{\Gamma}_{\lambda\gamma\delta}
  +
  \pdv{\tilde{x}^{\delta}}{x^{\beta}}\pdv{x^{\epsilon}}{\tilde{x}^{\delta}}
  \pdv{\tilde{x}^{\lambda}}{x^{\mu}}\pdv{\tilde{x}^{\gamma}}{x^{\epsilon}}{x^{\alpha}}
  g_{\lambda\gamma}
  \nonumber
  \\
   & \qquad
  +
  \pdv{\tilde{x}^{\gamma}}{x^{\alpha}}\pdv{x^{\epsilon}}{\tilde{x}^{\gamma}}
  \pdv{\tilde{x}^{\lambda}}{x^{\mu}}{x^{\epsilon}}
  \pdv{\tilde{x}^{\delta}}{x^{\beta}}
  g_{\lambda\delta}
  -
  \pdv{\tilde{x}^{\lambda}}{x^{\mu}}\pdv{x^{\epsilon}}{\tilde{x}^{\lambda}}
  \pdv{\tilde{x}^{\gamma}}{x^{\epsilon}}{x^{\alpha}}\pdv{\tilde{x}^{\delta}}{x^{\beta}}
  g_{\gamma\delta}
  .
\end{align}
(I think this result is somewhat strange.)


% ----------------------------------------------------------------------------------------------------
\clearpage
\section{Problem 2}

From the previous problem, we obtain the transformation law
\begin{equation}
  \tilde{\Gamma}^{\lambda}_{\ \mu\nu}
  =
  \pdv{\tilde{x}^{\lambda}}{x^{\gamma}}
  \pdv{x^{\alpha}}{\tilde{x}^{\mu}}
  \pdv{x^{\beta}}{\tilde{x}^{\nu}}
  \Gamma^{\gamma}_{\ \alpha\beta}
  +
  \pdv{\tilde{x}^{\lambda}}{x^{\gamma}}\pdv{x^{\gamma}}{\tilde{x}^{\mu}}{\tilde{x}^{\nu}}
  .
\end{equation}
Since we already know the transformation laws, what we have to do is just to compute them. Thus the transformation should be
\begin{align}
  \tilde{\nabla}_{\mu}\tilde{V}_{\nu}
   & \equiv
  \pdv{\tilde{V}_{\nu}}{\tilde{x}^{\mu}}
  -
  \tilde{\Gamma}^{\lambda}_{\ \mu\nu}\tilde{V}_{\lambda}
  \nonumber
  \\
   & =
  \pdv{x^{\alpha}}{\tilde{x}^{\mu}}\pdv{}{x^{\alpha}}\left( \pdv{x^{\beta}}{\tilde{x}^{\nu}}V_{\beta} \right)
  -
  \left(
  \pdv{\tilde{x}^{\lambda}}{x^{\gamma}}
  \pdv{x^{\alpha}}{\tilde{x}^{\mu}}
  \pdv{x^{\beta}}{\tilde{x}^{\nu}}
  \Gamma^{\gamma}_{\ \alpha\beta}
  +
  \pdv{\tilde{x}^{\lambda}}{x^{\gamma}}\pdv{x^{\gamma}}{\tilde{x}^{\mu}}{\tilde{x}^{\nu}}
  \right)
  \cdot
  \pdv{x^{\delta}}{\tilde{x}^{\lambda}}V_{\delta}
  \nonumber
  \\
   & =
  \cancel{
  \pdv{x^{\beta}}{\tilde{x}^{\mu}}{\tilde{x}^{\nu}}V_{\beta}
  }
  +
  \pdv{x^{\alpha}}{\tilde{x}^{\mu}}\pdv{x^{\beta}}{\tilde{x}^{\nu}}\pdv{V_{\beta}}{x^{\alpha}}
  -
  \pdv{\tilde{x}^{\lambda}}{x^{\gamma}}
  \pdv{x^{\alpha}}{\tilde{x}^{\mu}}
  \pdv{x^{\beta}}{\tilde{x}^{\nu}}
  \Gamma^{\gamma}_{\ \alpha\beta}
  \cdot
  \pdv{x^{\delta}}{\tilde{x}^{\lambda}}V_{\delta}
  -
  \cancel{
  \pdv{\tilde{x}^{\lambda}}{x^{\gamma}}\pdv{x^{\gamma}}{\tilde{x}^{\mu}}{\tilde{x}^{\nu}}
  \cdot
  \pdv{x^{\delta}}{\tilde{x}^{\lambda}}V_{\delta}
  }
  \nonumber
  \\
   & =
  \pdv{x^{\alpha}}{\tilde{x}^{\mu}}\pdv{x^{\beta}}{\tilde{x}^{\nu}}
  \left(
  \pdv{V_{\beta}}{x^{\alpha}}
  -
  \Gamma^{\gamma}_{\ \alpha\beta}V_{\gamma}
  \right)
  =
  \pdv{x^{\alpha}}{\tilde{x}^{\mu}}\pdv{x^{\beta}}{\tilde{x}^{\nu}}\nabla_{\alpha}V_{\beta}
\end{align}
and we finally attain
\begin{equation}  
  \tilde{\nabla}_{\mu}\tilde{V}_{\nu}
  =
  \pdv{x^{\alpha}}{\tilde{x}^{\mu}}\pdv{x^{\beta}}{\tilde{x}^{\nu}}\nabla_{\alpha}V_{\beta}
  .
\end{equation}



% ----------------------------------------------------------------------------------------------------
\clearpage
\section{Problem 3*}















% ----------------------------------------------------------------------------------------------------
\clearpage
\section{Problem 4}

Let us show the following formula\footnote{
  The exponential of matrix $A$ satisfies
  \begin{equation}
    \det e^{A}=e^{\Tr A}
    \nonumber
  \end{equation}
  and taking $A\equiv\ln g$, we find \eqref{eqn:4-1}.
}:
\begin{equation}
  \pdv{}{x^{\mu}}\sqrt{-g}
  =
  \sqrt{-g}\Gamma^{\lambda}_{\ \mu\lambda}
  .
  \label{eqn:4-1}
\end{equation}
Assuming this relation, we immediately reach the answer
\begin{align}
  \frac{1}{\sqrt{-g}}\pdv{}{x^{\lambda}}\left(\sqrt{-g}A^{\lambda}\right)
  &=
  \frac{1}{\sqrt{-g}}\left( \pdv{}{x^{\lambda}}\sqrt{-g} \right)A^{\lambda}
  +
  \pdv{A^{\lambda}}{x^{\lambda}}
  \nonumber
  \\
  &=
  \Gamma^{\sigma}_{\ \lambda\sigma}A^{\kappa}
  +
  \pdv{A^{\lambda}}{x^{\lambda}}
  =
  \nabla_{\lambda}A^{\lambda}
  .
\end{align}
So what is left is to prove the relation \eqref{eqn:4-1}.
\begin{proof}
  We will use the relation 
  \begin{equation}
    \ln g
    =
    \Tr \ln g
    \label{eqn:4-2}
  \end{equation}
  and take the derivative to $x^{\lambda}$. Then we get
  \begin{equation}
    \pdv{}{x^{\lambda}}\ln g
    =
    \pdv{}{x^{\lambda}}\Tr\ln g
    \label{eqn:4-3}
  \end{equation}
  and by computing both sides carefully, we can obtain
  \begin{equation}
    \frac{1}{g}\pdv{g}{x^{\lambda}}
    =
    g^{\alpha\beta}\pdv{g_{\alpha\beta}}{x^{\lambda}}
    .    
    \label{eqn:4-4}
  \end{equation} 
  Note that we use the relation 
  \begin{equation}
    \pdv{}{x^{\lambda}}\ln g_{\alpha\beta}
    =
    (g^{-1})_{\alpha\gamma}\pdv{g_{\gamma\beta}}{x^{\lambda}}
  \end{equation}
  when we derivate the RHS of \eqref{eqn:4-3}. Thus we find
  \begin{align}
    \pdv{}{x^{\lambda}}\sqrt{-g}
    &=
    -\pdv{g}{x^{\lambda}}
    \cdot
    \frac{1}{2}\frac{1}{\sqrt{-g}}
    \nonumber
    \\
    &=
    \frac{1}{2}\sqrt{-g}g^{\alpha\beta}\pdv{g_{\alpha\beta}}{x^{\lambda}}
  \end{align}
  by using \eqref{eqn:4-4}. On the other hand, the Christoffel symbol is defined as \eqref{eqn:christoffel_symbol} and contracting the indices, the relation holds
  \begin{equation}
    \Gamma^{\lambda}_{\ \mu\lambda}
    =
    \frac{1}{2}g^{\alpha\beta}\pdv{g_{\alpha\beta}}{x^{\lambda}}
  \end{equation}
  and finally we attain \eqref{eqn:4-1}.
\end{proof}



% ----------------------------------------
% \clearpage
% \appendix
% \section{Notes}

% ----------------------------------------
% \clearpage
% \bibliography{ref}
% \bibliographystyle{ytamsalpha}

% ----------------------------------------
% \clearpage
% \index{hoge@hoge}
% \printindex

\end{document}
